feat: finiteness of inversions of a permutation

Fifteen/Data/Permutation/Sign.lean
@@ -3,6 +3,8 @@ Copyright (c) 2023 Jun Yoshida. All rights reserved.
 Released under Apache 2.0 license as described in the file LICENSE.
 -/
 
+import Fifteen.Logic.BishopFin
+import Fifteen.Data.Nat.Basic
 import Fifteen.Data.Permutation.Basic
 
 /-!
@@ -46,23 +48,11 @@ instance (n : Nat) (x : Permutation n) : Repr (Inversion x) where
 
 end Inversion
 
-
-@[inline]
-private def _root_.Nat.foldM' {α : Type u} {m : Type u → Type v} [Monad m] (k : Nat) (f : Fin k → α → m α) (init : α) : m α :=
-  let rec @[specialize] loop : (i : Nat) → i ≤ k → α → m α
-    | 0       , _, a => pure a
-    | i'@(i+1), h, a =>
-      have : k-i' < k := by
-        cases ‹i' = i+1›; dsimp at h
-        exact Nat.sub_lt (trans i.zero_lt_succ h) i.zero_lt_succ
-      f ⟨k-i', this⟩ a >>= loop i (trans i.le_succ h)
-  loop k .refl init
-
 /-- Get the list of inversions of a permutation. -/
 @[inline]
 def inversions (x : Permutation n) : Array (Inversion x) :=
-  #[] |> Nat.foldM' (m:=Id) n fun j ivs =>
-    ivs |> Nat.foldM' j.1 fun i ivs =>
+  #[] |> Nat.fold' n fun j ivs =>
+    ivs |> Nat.fold' j.1 fun i ivs =>
       if h : x[i.1]'(Nat.lt_trans i.2 j.2) > x[j.1] then
         ivs.push {
           fst := i.castLE (Nat.le_of_lt j.2)
@@ -72,6 +62,95 @@ def inversions (x : Permutation n) : Array (Inversion x) :=
         }
       else
         ivs
+
+theorem mem_inversions (x : Permutation n) (iv : Inversion x) : iv ∈ x.inversions := by
+  let ⟨i,j,hlt,hinv⟩ := iv
+  dsimp [inversions]
+  refine Nat.fold'_induction (motive := fun k (ivs : Array (Inversion x)) => j.1 < k → ⟨i,j,hlt,hinv⟩ ∈ ivs) n _ #[] ?zero ?succ j.2
+  all_goals simp
+  . intro hj; cases hj
+  . intro k hk invs IH hjk
+    have : i.1 < k := trans (r:=LT.lt (α:=Nat)) hlt (Nat.le_of_succ_le_succ hjk)
+    refine Nat.fold'_induction (motive := fun l (ivs' : Array (Inversion x)) => (i.1 < l ∨ j.1 < k) → ⟨i,j,hlt,hinv⟩ ∈ ivs') k _ invs ?_ ?_ (Or.inl this)
+    all_goals simp
+    . intro hi
+      cases hi with
+      | inl hi => cases hi
+      | inr hj => exact IH hj
+    . intro l hl invs' IH' hil
+      cases Nat.eq_or_lt_of_le (Nat.le_of_succ_le_succ hjk) with
+      | inl heq =>
+        cases heq
+        have : i.1 ≤ l :=
+          Nat.le_of_succ_le_succ (Or.resolve_right hil j.1.lt_irrefl)
+        cases Nat.eq_or_lt_of_le this with
+        | inl heq =>
+          cases heq; rewrite [dif_pos hinv]
+          exact Array.mem_push.mpr <| Or.inr rfl
+        | inr hlt =>
+          specialize IH' (Or.inl hlt)
+          if hx : x[l]'(Nat.lt_trans hl j.2) > x[j.1] then
+            rewrite [dif_pos hx]
+            exact Array.mem_push.mpr <| Or.inl IH'
+          else
+            rewrite [dif_neg hx]; exact IH'
+      | inr hlt =>
+        specialize IH' (Or.inr hlt)
+        if hx : x[l]'(Nat.lt_trans hl hk) > x[k]'hk then
+          rewrite [dif_pos hx]
+          exact Array.mem_push.mpr <| Or.inl IH'
+        else
+          rewrite [dif_neg hx]; exact IH'
+
+theorem nodup_inversions (x : Permutation n) : x.inversions.Nodup := by
+  suffices x.inversions.Nodup ∧ ∀ iv, iv ∈ x.inversions → iv.snd.1 < n
+  from this.1
+  dsimp [inversions]
+  refine Nat.fold'_induction (motive := fun k (ivs : Array (Inversion x)) => ivs.Nodup ∧ ∀ iv, iv ∈ ivs → iv.snd.1 < k) n _ #[] ?_ ?_
+  all_goals simp
+  . exact ⟨.nil, fun _ h => nomatch h⟩
+  . intro k hk ivs ivs_nodup ivs_lt
+    generalize hivs' : Nat.fold' k _ ivs = ivs'
+    suffices Array.Nodup ivs' ∧ ∀ iv, iv ∈ ivs' → iv.snd.1 < k ∨ (iv.snd.1 = k ∧ iv.fst.1 < k) by
+      refine And.imp_right ?_ this
+      intro hivs' iv hiv
+      apply Nat.succ_le_succ; apply Nat.le_iff_lt_or_eq.mpr
+      exact Or.imp_right And.left (hivs' iv hiv)
+    cases hivs'
+    refine Nat.fold'_induction (motive := fun l (ivs' : Array (Inversion x)) => ivs'.Nodup ∧ ∀ iv, iv ∈ ivs' → iv.snd.1 < k ∨ (iv.snd.1 = k ∧ iv.fst.1 < l)) k _ ivs ?_ ?_
+    all_goals simp
+    . exact And.intro ivs_nodup fun iv hiv => Or.inl <| ivs_lt iv hiv
+    . intro l hl ivs' ivs'_nodup ivs'_lt
+      if hx : x[l]'(Nat.lt_trans hl hk) > x[k] then
+        simp only [dif_pos hx, Array.nodup_push, Array.mem_push, ivs'_nodup, true_and]
+        constructor
+        . intro h
+          specialize ivs'_lt _ h; dsimp at ivs'_lt
+          refine ivs'_lt.elim ?_ ?_
+          . exact Nat.lt_irrefl k
+          . intro h; exact Nat.lt_irrefl l h.2
+        . intro iv hiv
+          cases hiv with
+          | inl hmem =>
+            refine Or.imp_right ?_ <| ivs'_lt iv hmem
+            exact And.imp_right Nat.le.step
+          | inr heq =>
+            cases heq; dsimp
+            exact Or.inr ⟨rfl, l.lt_succ_self⟩
+      else
+        simp only [dif_neg hx]
+        apply And.intro ivs'_nodup
+        intro iv hiv; specialize ivs'_lt iv hiv
+        refine Or.imp_right ?_ ivs'_lt
+        exact And.imp_right Nat.le.step
+
+instance Inversion.finite (x : Permutation n) : BishopFin (Inversion x) where
+  elems' := x.inversions.toList
+  nodup_elems' := by
+    rewrite [Array.toList_eq]; exact x.nodup_inversions
+  mem_elems' := by
+    simp only [Array.toList_eq, ← Array.mem_iff_mem_data]
+    exact x.mem_inversions
 
 /--
 `Permutation.sign x` is the sign of the permutation `x : Permutation n`.
